theories/interop/wp_boundary_laws.v
@@ -28,8 +28,9 @@ Lemma wrap_interp_c_to_ml ws ρc mem θ vs lvs :
   GC θ -∗
   at_boundary wrap_lang -∗
   lvs ~~∗ vs -∗
-  ∃ ρml σ,
-  ⌜c_to_ml ws ρc mem vs ρml σ⌝ ∗
+  ∃ ρml σ ζ,
+  ⌜c_to_ml_heap ρc mem ρml σ ζ⌝ ∗
+  ⌜c_to_ml_vals ws ρc vs ρml ζ⌝ ∗
   |==> wrap_state_interp (Wrap.MLState ρml σ) ∗ not_at_boundary.
 Proof using.
   iIntros (Hlv) "Hσ HGC Hnb #Hblk".
@@ -46,15 +47,68 @@ Proof using.
   iDestruct (hgh_export_ml_heap with "GCHGH")
     as (ζ' χ' ζfreeze) "(GCHGH & Hσ & %Hχ & %Hfrz & %Hζ)".
   iAssert (⌜Forall2 (is_val χ' ζfreeze) vs lvs⌝)%I as %Hval.
-  { iDestruct (hgh_block_sim_is_val with "GCHGH Hblk") as %Hval. iPureIntro.
+  { iDestruct (hgh_block_sim_is_vals with "GCHGH Hblk") as %Hval. iPureIntro.
     eapply Forall2_impl; first done. intros ? ?. eapply is_val_mono; eauto.
     by eapply lstore_hybrid_repr_lstore_sub. }
 
   (* TODO: refactor opsem to use lstore_hybrid_repr? *)
   destruct Hζ as (ζσ&?&?&?&?).
-  iExists (WrapstateML _ _ _ _), _. iSplit.
-  { iPureIntro. unfold c_to_ml. cbn.
-    eexists σMLvirt, _, _, ζfreeze, ζσ. split_and!; eauto. by rewrite map_union_comm. }
+  iExists (WrapstateML _ _ _ _), _, _. iSplit. 2: iSplit.
+  { iPureIntro. unfold c_to_ml_heap. cbn.
+    eexists ζσ. split_and!; eauto. by rewrite map_union_comm. }
+  { iPureIntro. unfold c_to_ml_vals. cbn. exists lvs. split_and!; eauto. }
+
+  iMod (ghost_var_update_halves with "Hnb SIbound") as "(Hb & SIbound)".
+  iMod (ghost_var_update_halves with "GCζ SIζ") as "(GCζ & SIζ)".
+  iMod (ghost_var_update_halves with "GCχ SIχ") as "(GCχ & SIχ)".
+  iMod (ghost_var_update_halves with "GCθ SIθ") as "(GCθ & SIθ)".
+  iMod (ghost_var_update_halves with "GCroots SIroots") as "(GCroots & SIroots)".
+  iMod (set_to_none with "HσC GCrootspto") as "(HσC & GCrootspto)"; first done.
+
+  iModIntro. iSplitR "SIbound"; last by iFrame "SIbound".
+  rewrite /= /named. iFrame "Hσ".
+  unfold private_state_interp, ML_state_interp, GC_remnant, named; cbn.
+  iFrame. iPureIntro.
+  destruct Hpriv as (mem_r & ->%repr_roots_dom & Hpriv2 & Hpriv3); by apply map_disjoint_dom.
+Qed.
+
+Lemma wrap_interp_c_to_ml_out ow ρc mem θ ov olv :
+  repr_lval_out θ olv ow →
+  wrap_state_interp (Wrap.CState ρc mem) -∗
+  GC θ -∗
+  at_boundary wrap_lang -∗
+  olv ~~ₒ ov -∗
+  ∃ ρml σ ζ,
+  ⌜c_to_ml_heap ρc mem ρml σ ζ⌝ ∗
+  ⌜c_to_ml_outcome ow ρc ov ρml ζ⌝ ∗
+  |==> wrap_state_interp (Wrap.MLState ρml σ) ∗ not_at_boundary.
+Proof using.
+  iIntros (Hlv) "Hσ HGC Hnb Hblk".
+  iNamed "Hσ". iNamed "SIC". iNamed "HGC". simplify_eq. SI_GC_agree.
+
+  iAssert (⌜∀ k lv, roots_m !! k = Some lv →
+            ∃ w, mem !! k = Some (Storing w) ∧ repr_lval (θC ρc) lv w⌝)%I as "%Hroots".
+  1: { iIntros (kk vv Hroots).
+       iPoseProof (big_sepM_lookup with "GCrootspto") as "(%wr & Hwr & %Hw2)"; first done.
+       iExists wr. iSplit; last done. iApply (gen_heap_valid with "HσC Hwr"). }
+  apply map_Forall_lookup_2 in Hroots.
+  destruct (make_repr (θC ρc) roots_m mem) as [privmem Hpriv]; try done; [].
+
+  iDestruct (hgh_export_ml_heap with "GCHGH")
+    as (ζ' χ' ζfreeze) "(GCHGH & Hσ & %Hχ & %Hfrz & %Hζ)".
+  iAssert (⌜is_val_out χ' ζfreeze ov olv⌝)%I as %Hval.
+  { iDestruct (hgh_block_sim_is_out with "GCHGH Hblk") as %Hval. iPureIntro.
+    eapply (is_val_out_mono χ' χ' ζ'); eauto.
+    by eapply lstore_hybrid_repr_lstore_sub. }
+
+  destruct Hζ as (ζσ&?&?&?&?).
+  (* TODO: refactor opsem to use lstore_hybrid_repr? *)
+  iExists (WrapstateML _ _ _ _), _, _. iSplit. 2: iSplit.
+  { iPureIntro. unfold c_to_ml_outcome. cbn.
+    eexists ζσ. split_and!; eauto;
+    first by rewrite map_union_comm. }
+  { iPureIntro. unfold c_to_ml_outcome. cbn.
+    exists olv. split; eauto. }
 
   iMod (ghost_var_update_halves with "Hnb SIbound") as "(Hb & SIbound)".
   iMod (ghost_var_update_halves with "GCζ SIζ") as "(GCζ & SIζ)".
@@ -71,7 +125,8 @@ Proof using.
 Qed.
 
 Lemma wrap_interp_ml_to_c vs ρml σ ws ρc mem :
-  ml_to_c_core vs ρml σ ws ρc mem →
+  ml_to_c_heap ρml σ ρc mem →
+  (∃ lvs, Forall2 (repr_lval (θC ρc)) lvs ws ∧ Forall2 (is_val (χC ρc) (ζC ρc)) vs lvs) →
   wrap_state_interp (Wrap.MLState ρml σ) -∗
   not_at_boundary
   ==∗
@@ -80,10 +135,11 @@ Lemma wrap_interp_ml_to_c vs ρml σ ws ρc mem :
   GC (θC ρc) ∗
   (∃ lvs, lvs ~~∗ vs ∗ ⌜Forall2 (repr_lval (θC ρc)) lvs ws⌝).
 Proof using.
-  iIntros (Hml_to_c) "Hst Hb".
-  destruct Hml_to_c as (ζσ & ζnewimm & lvs & HH).
+  iIntros (Hml_to_c Hlvs) "Hst Hb".
+  destruct Hlvs as (lvs & Hrepre & Hisval).
+  destruct Hml_to_c as (ζσ & ζnewimm & HH).
   destruct HH as (Hmono & Hblocks & Hprivblocks & HζC & Hζdisj &
-                    Hstore & Hvals & ? & ? & ? & Hroots & ?).
+                    Hstore & ? & ? & Hroots & ?).
 
   iNamed "Hst". iNamed "SIML". iNamed "SIGCrem".
   iDestruct (hgh_dom_lstore_sub with "GCHGH") as %Hζsub.
@@ -104,13 +160,58 @@ Proof using.
     { eapply is_store_blocks_lstore_dom_sub; eauto. }
     { eapply is_private_blocks_dom_sub; eauto. } }
   iMod (set_to_some with "HσCv GCrootspto") as "(HσCv & GCrootspto)"; first done.
-  iDestruct (hgh_block_sim_of _ _ _ vs lvs with "GCHGH") as "#Hsim"; first eassumption.
+  iDestruct (hgh_block_sim_of_vals _ _ _ vs lvs with "GCHGH") as "#Hsim"; first eassumption.
 
   iModIntro. iFrame "Hnb". rewrite /= /named.
   iFrame "HσCv SIζ SIχ SIθ SIroots SIbound".
   iSplitL "SIinit". { iExists false. iFrame. } iSplit.
   { rewrite /GC /named. iExists _, _, _, _, _. iFrame. iPureIntro; split_and!; eauto. }
   { iExists _; by iFrame "Hsim". }
+Qed.
+
+Lemma wrap_interp_ml_to_c_out ov ρml σ ow ρc mem :
+  ml_to_c_heap ρml σ ρc mem →
+  ml_to_c_outcome ov ow ρc →
+  wrap_state_interp (Wrap.MLState ρml σ) -∗
+  not_at_boundary
+  ==∗
+  wrap_state_interp (Wrap.CState ρc mem) ∗
+  at_boundary wrap_lang ∗
+  GC (θC ρc) ∗
+  (∃ olv, olv ~~ₒ ov ∗ ⌜repr_lval_out (θC ρc) olv ow⌝).
+Proof using.
+  iIntros (Hml_to_c H) "Hst Hb".
+  destruct H as (lv & Hval & Hrepre).
+  destruct Hml_to_c as (ζσ & ζnewimm & HH).
+  destruct HH as (Hmono & Hblocks & Hprivblocks & HζC & Hζdisj &
+                    Hstore & ? & ? & Hroots & ?).
+
+  iNamed "Hst". iNamed "SIML". iNamed "SIGCrem".
+  iDestruct (hgh_dom_lstore_sub with "GCHGH") as %Hζsub.
+  iMod (ghost_var_update_halves with "Hb SIbound") as "(Hnb & SIbound)".
+  iMod (ghost_var_update_halves with "SIζ GCζ") as "(SIζ & GCζ)".
+  iMod (ghost_var_update_halves with "SIχ GCχ") as "(SIχ & GCχ)".
+  iMod (ghost_var_update_halves with "SIθ GCθ") as "(SIθ & GCθ)".
+  iMod (ghost_var_update_halves with "SIroots GCroots") as "(SIroots & GCroots)".
+  apply map_disjoint_union_r in Hζdisj as [Hζdisj1 Hζdisj2].
+  iMod (hgh_import_ml_interp _ _ _ _ (ζC ρc) with "GCHGH HσML") as "GCHGH"; eauto.
+  (* TODO: use lstore_hybrid_repr in the opsem? *)
+  { exists ζσ. split_and!; eauto.
+    { rewrite map_union_assoc. rewrite (map_union_comm ζσ); first done. by symmetry. }
+    { apply map_disjoint_union_r; split; eauto.
+      by eapply is_store_blocks_is_private_blocks_disjoint. } }
+  { rewrite HζC !dom_union_L. repeat apply union_least.
+    { destruct Hmono as [?%subseteq_dom ?]. set_solver. }
+    { eapply is_store_blocks_lstore_dom_sub; eauto. }
+    { eapply is_private_blocks_dom_sub; eauto. } }
+  iMod (set_to_some with "HσCv GCrootspto") as "(HσCv & GCrootspto)"; first done.
+  iDestruct (hgh_block_sim_of_out _ _ _ ov lv with "GCHGH") as "#Hsim"; first eassumption.
+
+  iModIntro. iFrame "Hnb". rewrite /= /named.
+  iFrame "HσCv SIζ SIχ SIθ SIroots SIbound".
+  iSplitL "SIinit". { iExists false. iFrame. } iSplit.
+  { rewrite /GC /named. iExists _, _, _, _, _. iFrame. iPureIntro; split_and!; eauto. }
+  { iExists lv. iSplit; eauto. }
 Qed.
 
 End BoundaryLaws.
