theories/interop/wp_prims/isblock.v
@@ -30,7 +30,7 @@ Proof using.
   SI_at_boundary. iNamed "HGC". SI_GC_agree.
 
   iApply wp_pre_cases_c_prim; [done..|].
-  iExists (λ '(e', σ'), e' = WrSE (ExprV #(match lv with  Lint _ => 0 | Lloc _ => 1 end)) ∧ σ' = CState ρc mem).
+  iExists (λ '(e', σ'), e' = WrSE (ExprO (OVal #(match lv with  Lint _ => 0 | Lloc _ => 1 end))) ∧ σ' = CState ρc mem).
   iSplit. { iPureIntro; edestruct lv; try (econstructor; eauto; fail). }
   iIntros (? ? ? (? & ?)); simplify_eq.
   do 3 iModIntro. iFrame. iSplitL "SIinit". { iExists false. iFrame. }
