theories/interop/wp_prims/read_foreign.v
@@ -35,7 +35,7 @@ Proof using.
   }
   destruct Helem2 as [m' Helem2].
   iApply wp_pre_cases_c_prim; [done..|].
-  iExists (λ '(e', σ'), e' = WrSE (ExprV w') ∧ σ' = CState ρc mem).
+  iExists (λ '(e', σ'), e' = WrSE (ExprO (OVal w')) ∧ σ' = CState ρc mem).
   iSplit. { iPureIntro; econstructor; eauto. }
   iIntros (? ? ? (? & ?)); simplify_eq.
   do 3 iModIntro. iFrame. iSplitL "SIinit". { iExists false. iFrame. }
