theories/interop/wp_simulation.v
@@ -36,9 +36,9 @@ Proof using.
   iIntros "%st SI".
   iDestruct (SI_not_at_boundary_is_in_ML with "SI Hnb") as "%H"; destruct H as (ρml & σ & ->).
   iModIntro. iRight. iRight.
-  iSplit; first done.
 
-  iAssert (⌜ml_to_c [v] ρml σ (λ ws ρc mem, ml_to_c_core [v] ρml σ ws ρc mem)⌝)%I as "%Hprog".
+  iSplit; first done.
+  iAssert (⌜sanity_check ρml σ⌝)%I as "%Hprog".
   { iNamed "SI". iNamed "SIML". iNamed "SIGCrem".
     iDestruct (hgh_discarded_locs_pub with "GCHGH HσML") as %?.
     iDestruct (hgh_dom_lstore_sub with "GCHGH") as %?.
@@ -46,18 +46,23 @@ Proof using.
     iPureIntro; split_and!; eauto. }
 
   iExists (λ '(e', σ'), ∃ w ρc mem,
-    ml_to_c_core [v] ρml σ [w] ρc mem ∧
-    e' = WrSE (ExprV w) ∧ σ' = CState ρc mem).
-  iSplit. { iPureIntro. eapply ValS; naive_solver. }
+    ml_to_c_heap ρml σ ρc mem ∧
+    ml_to_c_outcome (OVal v) (OVal w) ρc ∧
+    e' = WrSE (ExprO (OVal w)) ∧ σ' = CState ρc mem).
+  iSplit. { iPureIntro. eapply OutS; try naive_solver.
+    intros * Hp (lv & Hval & Hrepr). inversion Hval; subst.
+    inversion Hrepr; subst. exists v0, ρc, mem.
+    split_and!; try naive_solver. unfold ml_to_c_outcome. now exists (OVal lv0). }
 
-  iIntros (? ? (w & ρc & mem & Hcore & -> & ->)).
-  iMod (wrap_interp_ml_to_c with "SI Hnb") as "(SI & Hb & HGC & (%lvs & Hsim & %Hrepr))";
-    first done.
+  iIntros (? ? (w & ρc & mem & Hout & Hcore & -> & ->)).
+  iMod (wrap_interp_ml_to_c_out with "SI Hnb") as "(SI & Hb & HGC & H)";
+    first done; first done.
   do 3 iModIntro. iFrame "SI".
-  replace (WrSE (ExprV w)) with (of_outcome wrap_lang (OVal w)) by done. 
+  replace (WrSE (ExprO (OVal w))) with (of_outcome wrap_lang (OVal w)) by done.
   iApply weakestpre.wp_outcome'.
-  iDestruct (big_sepL2_cons_inv_l with "Hsim") as "(% & % & -> & Hsim & _)".
-  iExists _, _, _. iFrame. by inversion Hrepr; simplify_eq.
+  iDestruct "H" as "(% & Hls & %Hval)".
+  inversion Hval; subst.
+  iExists _, w, lv. iFrame. repeat iSplit; eauto.
 Qed.
 
 Lemma wp_simulates (Ψ : protocol ML_lang.val Σ) eml emain Φ :
@@ -99,20 +104,23 @@ Proof.
 
     iModIntro. iRight; iRight.
     iSplit; first done.
-    iExists (λ '(e', σ'), ∃ ws ρc mem,
-      ml_to_c_core vs ρml σ ws ρc mem ∧
+    iExists (λ '(e', σ'), ∃ ws ρc mem lvs,
+      Forall2 (is_val (χC ρc) (ζC ρc)) vs lvs ∧
+      Forall2 (repr_lval (θC ρc)) lvs ws ∧
+      ml_to_c_heap ρml σ ρc mem ∧
       e' = WrE (Wrap.ExprCall fn_name ws) [K'] ∧
       σ' = CState ρc mem).
     iSplit.
     { iPureIntro.
-      eapply MakeCallS with (YC := (λ ws ρc mem, ml_to_c_core vs ρml σ ws ρc mem)); eauto.
+      eapply MakeCallS; eauto.
       { done. }
       { apply not_elem_of_dom. rewrite dom_wrap_prog not_elem_of_prim_names //. }
       { split_and!; eauto. }
-      { intros. do 3 eexists. split_and!; eauto. } }
-    iIntros (? ? (ws & ρc & mem & Hcore & -> & ->)).
-    iMod (wrap_interp_ml_to_c with "[- Hnb Hr HT] Hnb") as "(Hσ & Hb & HGC & (%lvs & #Hblk & %))";
+      { intros * Hep (lvs & ? & ?). do 4 eexists. split_and!; eauto. } }
+    iIntros (? ? (ws & ρc & mem & lvs & ? & ? & Hcore & -> & ->)).
+    iMod (wrap_interp_ml_to_c with "[- Hnb Hr HT] Hnb") as "(Hσ & Hb & HGC & (%lv & #Hblk & %))";
       first done.
+    { exists lvs; split_and; eauto.  }
     { rewrite /wrap_state_interp /ML_state_interp /named.
       iSplitL "Hσ"; first by iFrame. by iFrame. }
     do 3 iModIntro. iFrame "Hσ".
@@ -143,9 +151,10 @@ Proof.
     iDestruct (SI_at_boundary_is_in_C with "Hst' Hb") as %(ρc'&mem'&->). simpl.
     iRight; iRight. iSplit; first done.
 
-    iDestruct (wrap_interp_c_to_ml with "Hst' HGC Hb [Hsim]") as (ρml' σ' Hc_to_ml) "HH".
-    2: by iApply big_sepL2_singleton.
-    1: by constructor.
+    iDestruct ((wrap_interp_c_to_ml_out (OVal wret) _ _ _ (OVal vret) (OVal lvret)) with "Hst' HGC Hb [Hsim]")
+      as (ρml' σ' ζ Hc_to_ml_heap Hc_to_ml_out) "HH".
+    { constructor. eauto. }
+    { cbn. iFrame. }
     iExists (λ '(e2, σ2),
       e2 = WrSE (ExprML (language.fill K' (Val vret))) ∧
       σ2 = MLState ρml' σ').
@@ -199,7 +208,7 @@ Proof using.
 
   iDestruct "Hclos" as "#Hclos".
   iDestruct (wrap_interp_c_to_ml [w;w'] _ _ _ [RecV f x e; v']
-    with "Hst HGC Hb [Hclos Hsim']") as (ρml' σ' Hc_to_ml) "HH".
+    with "Hst HGC Hb [Hclos Hsim']") as (ρml' σ' ζ Hc_to_ml_heap Hc_to_ml_vals) "HH".
   { repeat constructor; eauto. }
   { iApply big_sepL2_cons. iSplit.
     { cbn. iExists _. by iFrame "Hclos". }
